Progress on teq_node_disj, Refactor stuff

uniana/cfg/CncLoop.v
@@ -2,20 +2,26 @@ Require Export CFGinnermost.
 
 (** cnc & ocnc **)
 
-Definition cnc_loop `{C : redCFG} s q s'
-  := loop_contains s' s /\ ~ deq_loop q s'.
+Definition cnc_loop `{C : redCFG} h p q
+  := loop_contains h p /\ ~ deq_loop q h.
 
-Definition ocnc_loop `{C : redCFG} s q s'
-  := cnc_loop s q s' /\ forall x, cnc_loop s q s' -> deq_loop x s'.
+Definition ocnc_loop `{C : redCFG} h p q
+  := cnc_loop h p q /\ forall h', loop_contains h' p -> deq_loop h' h.
 
+(*
 (* the ocnc loop has an exit such that q is deeper or equal to the exit *)
 Lemma ocnc_loop_exit `(C : redCFG) s q s'
       (Hocnc : ocnc_loop s q s')
   : exists e : Lab, exited s' e /\ deq_loop q e.
 Admitted.
+ *)
 
-Lemma ex_ocnc_loop `(C : redCFG) s q
-      (Hndeq : ~ deq_loop q s)
-  : exists s', ocnc_loop s q s'.
+Lemma ex_ocnc_loop `(C : redCFG) p q
+      (Hndeq : ~ deq_loop q p)
+  : exists h, ocnc_loop h p q .
 Admitted.
- 
+
+Lemma ocnc_depth `(C : redCFG) h p q
+      (Hocnc : ocnc_loop h p q)
+  : depth h = S (depth q).
+Admitted.
