uniana/disj/SpathIncl.v
@@ -1,15 +1,6 @@
 Require Export DiamondPaths.
 Require Import Lia.
 
-Definition sub_tag i j := |i| = |j| /\ hd 0 i <= hd 0 j /\ tl i = tl j.
-
-Lemma Tagle_len: forall [i j : Tag], i ⊴ j -> | i | = | j |.
-Proof.
-  intros. destruct H.
-  - eapply Taglt_len;eauto.
-  - subst. reflexivity.
-Qed.
-
 Lemma spath_jj_subtag `(SplitPaths)
       (Hjle : j1 ⊴ j2)
   : sub_tag j1 j2.
@@ -31,158 +22,6 @@ Proof.
 Qed.
 
 Hint Resolve jj_subtag : diamond.
-
-Lemma loop_tag_dom_eq `(C : redCFG) (h p : Lab) (i j : Tag) t
-      (Hloop : loop_contains h p)
-      (Hpath : TPath (root,start_tag) (p,i) t)
-      (Htagle : j = take_r (depth h) i)
-      (Hdep : |j| = depth h)
-  : (h,j) ∈ t.
-Proof.
-  subst j.
-  clear Hdep.
-  revert h p i Hloop Hpath.
-  induction t;intros.
-  + inv Hpath.
-  + unfold TPath in Hpath. path_simpl' Hpath. destruct t.
-    {
-      eapply path_single in Hpath. destruct Hpath.
-      inversion H. subst p i. eapply root_no_loop in Hloop. contradiction.
-    }
-    inv_path Hpath. destruct c as [q j].
-    specialize (IHt) with (p:=q) (i:=j).
-    eapply tcfg_edge_destruct' in H0.
-    destruct H0 as [H0|[H0|[H0|H0]]].
-    all: destruct H0 as [Htag Hedge].
-    * subst. right.
-      eapply IHt. all:cycle 1.
-      -- eapply H.
-      -- eapply basic_edge_eq_loop in Hedge. rewrite Hedge. assumption.
-    * eapply deq_loop_entry_or in Hedge;eauto.
-      destruct Hedge.
-      -- subst. right.
-         rewrite take_r_cons_drop.
-         2: {
-           eapply loop_contains_deq_loop in H0.
-           eapply tag_depth' in H. rewrite H.
-           eapply deq_loop_depth;eauto.
-         }
-         eapply IHt;eauto.
-      -- subst p. left. rewrite take_r_geq;eauto.
-         eapply tag_depth' in Hpath. lia.
-    * destruct j.
-      {
-        eapply tag_depth' in H. cbn in H. eapply loop_contains_depth_lt in Hloop.
-        eapply back_edge_eq_loop in Hedge. rewrite Hedge in H. lia.
-      }
-      cbn in Htag. subst i.
-      decide (h = p).
-      -- subst p. left. rewrite take_r_geq;eauto.
-         eapply tag_depth' in Hpath. lia.
-      -- right. rewrite take_r_cons_replace with (b:=n).
-         2: {
-           copy Hedge Hedge'.
-           eapply back_edge_eq_loop in Hedge.
-           copy Hloop Hloop'.
-           eapply loop_contains_deq_loop in Hloop.
-           eapply eq_loop1 in Hloop;eauto. 2: symmetry;eauto.
-           eapply tag_depth' in H.
-           enough (depth h < S (| j |)).
-           { cbn in H. rewrite H in H0. lia. }
-           eapply deq_loop_depth in Hloop.
-           eapply le_lt_or_eq in Hloop.
-           destruct Hloop.
-           ++ cbn in H. lia.
-           ++ exfalso. rewrite Hedge in H0.
-              eapply loop_contains_deq_loop in Hloop' as Hdeq.
-              eapply deq_loop_depth_eq in H0;eauto.
-              eapply n0. eapply head_unique;eauto.
-              ** eapply loop_contains_ledge;eauto.
-              ** split;eauto.
-         }
-         eapply IHt;eauto.
-         eapply back_edge_eq_loop in Hedge. rewrite Hedge. eauto.
-    * subst.
-      destruct j.
-      {
-        eapply tag_depth' in H. cbn in H. eapply loop_contains_depth_lt in Hloop.
-        destruct Hedge. eapply deq_loop_exited in H0. eapply deq_loop_depth in H0. lia.
-      }
-      right. rewrite <-take_r_cons_drop with (a:=n).
-      all: cbn.
-      2: {
-        eapply tag_depth' in H. cbn in H.
-        enough (depth h < S (|j|)) by lia.
-        rewrite H.
-        eapply depth_exit in Hedge.
-        eapply loop_contains_deq_loop in Hloop. eapply deq_loop_depth in Hloop.
-        lia.
-      }
-      eapply IHt;eauto.
-      destruct Hedge. eapply deq_loop_exited in H0. eapply H0. eauto.
-Qed.
-
-Lemma loop_tag_dom_same `(C : redCFG) (h : Lab) (i j : Tag) t
-      (Hloop : loop_head h)
-      (Hpath : TPath (root,start_tag) (h,i) t)
-      (Htagle : sub_tag j i)
-  : (h,j) ∈ t.
-Proof.
-  destruct Htagle as [Hlen [Hhd Htl]].
-  destruct i,j;cbn in *;[|congruence|congruence|].
-  { eapply tag_depth' in Hpath. cbn in Hpath. eapply depth_loop_head in Hloop. lia. }
-  subst j. clear Hlen.
-  revert t Hpath.
-  induction Hhd;intros.
-  - eapply path_contains_front;eauto.
-  - destruct t;[inv Hpath|].
-    unfold TPath in Hpath. path_simpl' Hpath.
-    inversion Hpath. subst.
-    destruct b as [q j].
-    eapply tcfg_edge_destruct' in H3.
-      destruct H3 as [H3|[H3|[H3|H3]]].
-      all: destruct H3 as [Htag Hedge].
-      * eapply basic_edge_no_loop2 in Hedge. contradiction.
-      * inv Htag.
-      * destruct j;cbn in Htag;[congruence|].
-        inv Htag.
-        right.
-        eapply loop_tag_dom_eq in H0 as Hel2;cycle 1.
-        -- eapply loop_contains_ledge;eassumption.
-        -- rewrite take_r_geq;eauto. eapply tag_depth' in H0. rewrite H0.
-           eapply back_edge_eq_loop in Hedge. rewrite Hedge. eauto.
-        -- eapply back_edge_eq_loop in Hedge. rewrite <-Hedge. eapply tag_depth' in H0. eauto.
-        -- eapply path_to_elem in Hel2;eauto. destructH.
-           eapply prefix_incl;[eauto|].
-           eapply IHHhd;eassumption.
-      * destruct j;cbn in Htag;[congruence|]. subst j. destruct Hedge.
-        eapply no_exit_head in H. contradiction.
-Qed.
-
-(* could be generalized with sub_tag _ _  -> sub_tag _ _ \/ Prefix _ _ *)
-Lemma loop_tag_dom `(C : redCFG) (h p : Lab) (i j : Tag) t
-      (Hloop : loop_contains h p)
-      (Hpath : TPath (root,start_tag) (p,i) t)
-      (Hstag : sub_tag j (take_r (depth h) i))
-      (Hdep : |j| = depth h)
-  : (h,j) ∈ t.
-Proof.
-  assert (depth h <= | i |) as Hdepi.
-  {
-    eapply tag_depth' in Hpath. rewrite Hpath.
-    eapply deq_loop_depth.
-    eapply loop_contains_deq_loop;eauto.
-  }
-  eapply loop_tag_dom_eq in Hpath as Hel2.
-  3: reflexivity.
-  2: eauto.
-  2: rewrite take_r_length_le;eauto.
-  eapply path_to_elem in Hel2;eauto.
-  destructH.
-  eapply prefix_incl;eauto.
-  eapply loop_tag_dom_same;eauto.
-  eapply loop_contains_loop_head;eauto.
-Qed.
 
 Hint Resolve Spath1 Spath2 Sdisj Sloop Stl Slen : spath.
 
@@ -418,4 +257,28 @@ Proof.
   setoid_rewrite Sloop.
   eapply spath_r1_incl_head_q.
   eapply SplitPaths_sym;eauto.
+Qed.
+
+Lemma spath_tag_eq1 `(S : SplitPaths)
+      (Hjle : j1 ⊴ j2)
+  : forall j, j ∈ map snd r1 -> take_r (depth q1) j = j1.
+Proof.
+  intros. destruct r1;[contradiction|].
+  specialize Spath1 as Hpath1.
+  unfold TPath in Hpath1. cbn in Hpath1. path_simpl' Hpath1.
+  eapply in_snd in H. destructH.
+  eapply path_rcons_inv' in Hpath1 as Hpath1'. destructH. destruct p0 as [u1 l1].
+  eapply path_to_elem in H as Hϕ;eauto. destructH.
+  eapply tpath_deq_no_haed_tag_eq in Hϕ0.
+  - eapply tpath_deq_no_haed_tag_eq in Hpath1'0;eauto with spath.
+    + erewrite <-take_r_geq.
+      * rewrite Hpath1'0. eapply Hϕ0.
+      * erewrite spath_j_len1;eauto.
+    + eapply tcfg_edge_depth_iff in Hpath1'1. eapply Hpath1'1;eauto with spath.
+    + intros. eapply spath_r1_incl_head_q;eauto.
+    + intros. eapply spath_no_back;eauto.
+  - eapply tcfg_edge_depth_iff in Hpath1'1. eapply Hpath1'1;eauto with spath.
+  - intros. eapply spath_r1_incl_head_q;eauto. eapply prefix_incl;eauto.
+    eapply prefix_map_fst;eauto.
+  - intros. eapply spath_no_back;eauto. eapply prefix_incl;eauto. eapply prefix_map_fst;eauto.
 Qed.
