uniana/disj/TeqPaths.v
@@ -1,7 +1,91 @@
-Require Export DiamondIncl.
+Require Export DiamondIncl CncLoop.
+Require Import Lia.
+
+Lemma only_inner_heads_tag_prefix `(C : redCFG) p i q j l
+      (Hdep : | i | = depth p)
+      (Hpath : TPath (p, i) (q, j) l)
+      (Hnhead : forall (h' : Lab) (k' : Tag), (h',k') ∈ tl (rev l) -> loop_contains h' q -> False)
+      (Hdeqq : forall (h' : Lab) (k' : Tag), (h',k') ∈ l -> deq_loop h' q)
+  : Prefix j i.
+Proof.
+  clear - Hpath Hnhead Hdeqq Hdep.
+  remember (l) as l' in Hpath.
+  assert (Postfix l' l) as Hpost by (rewrite Heql';econstructor;eauto).
+  assert ((p,i) ∈ l') as Hel.
+  { (rewrite Heql';eapply path_contains_back;subst;eauto). }
+  remember p as p'. remember i as i'. rewrite Heqp' in Hpath. rewrite Heqi' in Hpath.
+  rewrite Heqp' in Hdep. rewrite Heqi' in Hdep.
+  clear Heql' Heqp' Heqi'.
+  revert p' i' Hel p i Hpath Hdep.
+  rinduction l'.
+  - contradiction.
+  - eapply In_rcons in Hel. destruct Hel.
+    + subst a.
+      specialize (rcons_destruct l0) as Hl0. destruct Hl0;[|destructH];subst l0.
+      * cbn in *.
+        inversion Hpath;subst. 2: { inversion H4. }
+        destruct l;[inversion Hpost;congruence'|]; eapply postfix_hd_eq in Hpost;
+                                 inversion Hpost;subst;cbn.
+        econstructor;auto.
+      * destruct a.
+        unfold TPath in Hpath.
+        assert ((p',i') ∈ l) as Helpi.
+        { eapply postfix_incl;eauto. }
+        replace i' with (snd (p',i')) by (cbn;auto).
+        path_simpl' Hpath. cbn. copy Hpath Hpath'.
+        eapply path_nlrcons_edge in Hpath.
+        exploit' H.
+        1: { eapply postfix_step_left;eauto. }
+        specialize (H e t). exploit' H. specialize (H e t). exploit H.
+        1: eapply path_rcons_rinv;eauto.
+        1: eapply tcfg_edge_depth_iff in Hpath;eapply Hpath;eauto.
+        eapply tcfg_edge_destruct in Hpath as Q.
+        assert ((e,t) ∈ l) as Helet.
+        { eapply postfix_incl;eauto. }
+        destruct Q as [Q|[Q|[Q|Q]]]. all: subst.
+        -- eauto. (* normal *)
+        -- inversion H;subst. (* entry *)
+           ++ exfalso.
+              specialize (Hdeqq p i). exploit Hdeqq.
+              eapply deq_loop_depth in Hdeqq.
+              assert (|i| < |0 :: i|) as Q by (cbn;lia). clear Helet.
+              eapply tag_depth_unroot in Hpath';eauto. lia.
+           ++ auto.
+        -- inversion H.  (* back_edge *)
+           ++ subst.
+              destruct i. 1:cbn;econstructor.
+              exfalso.
+              eapply Hnhead.
+              ** eapply postfix_rev_prefix in Hpost.
+                 rewrite rev_rcons in Hpost.
+                 eapply prefix_tl in Hpost.
+                 eapply prefix_incl;eauto. rewrite rev_rcons. left. reflexivity.
+              ** specialize (tag_back_edge_iff Hpath) as [Q _]. exploit Q;eauto.
+                 eapply deq_loop_head_loop_contains.
+                 --- eapply deq_loop_depth_eq.
+                     +++ eapply Hdeqq;eauto.
+                     +++ eapply tag_depth_unroot in Hpath';eauto. cbn in Hpath',Hdep.
+                         eapply back_edge_eq_loop in Q. rewrite <-Q. lia.
+                 --- exists p;eauto.
+           ++ subst. destruct i.
+              ** cbn in H0. congruence.
+              ** inversion H0. subst. econstructor. eauto.
+        -- clear - H;destruct i;cbn in *;[auto|]. inversion H;subst;econstructor;auto.
+    + destruct l0;[cbn in *;contradiction|].
+      unfold TPath in Hpath. path_simpl' Hpath. cbn in Hpath. path_simpl' Hpath.
+      eapply tag_depth_unroot in Hpath as Hdepq;eauto.
+      eapply path_rcons_inv in Hpath. destructH. destruct p0.
+      eapply H;eauto.
+      * eapply postfix_step_left;eauto.
+      * eapply tag_depth_unroot2 in Hpath;eauto.
+Qed.
 
 Section teq.
   Context `(T : TeqPaths).
+
+  Lemma teq_split
+    : exists s k r1' r2', SplitPaths s q1 q2 k j1 j2 (r1 ++ r1') (r2 ++ r2').
+  Admitted.
 
   Lemma teq_no_back : forall x : Lab, x ∈ (q1 :: map fst r1) -> ~ loop_contains x q1.
   Admitted.
@@ -15,6 +99,10 @@ Section teq.
   Admitted.
 
   Lemma teq_r2_incl_head_q : forall x, x ∈ (q2 :: map fst r2) -> deq_loop x q1.
+  Admitted.
+
+  Lemma teq_tag_eq1
+    : forall j, j ∈ map snd r1 -> take_r (depth q1) j = j1.
   Admitted.
 
   Lemma teq_u1_deq_q
@@ -59,12 +147,10 @@ Section teq.
   Proof.
   Admitted.
 
-  Lemma teq_node_disj
-        (Hjeq : j1 = j2)
-    : Disjoint (q1 :: map fst r1) (q2 :: map fst r2).
-  Admitted.
-
 End teq.
+
+Hint Resolve Tpath1 Tpath2 Tdisj Tloop Tjj_len Ttl_eq Tlj_eq1 Tlj_eq2 Tj_len : teq.
+Hint Resolve teq_r1_incl_head_q teq_r2_incl_head_q teq_u1_deq_q teq_u2_deq_q Tloop : teq.
 
 Lemma TeqPaths_sym `(C : redCFG) u1 u2 q1 q2 l1 l2 j r1 r2
       (T : TeqPaths u1 u2 q1 q2 l1 l2 j j r1 r2)
@@ -82,5 +168,96 @@ Proof.
   - destruct Tlj_eq1;[left|right];firstorder.
   - rewrite <-Tloop. eauto.
 Qed.
-
-Hint Resolve teq_r1_incl_head_q teq_r2_incl_head_q teq_u1_deq_q teq_u2_deq_q Tloop : teq.
+Lemma ex_outermost `(C : redCFG) p q
+      (Hdeq : deq_loop p q)
+      (Hndeq : ~ deq_loop q p)
+  : exists h, loop_contains h p /\ ~ loop_contains h q /\ forall h', deq_loop h h' -> loop_contains h' h.
+Lemma teq_node_disj `(T : TeqPaths)
+      (Hjeq : j1 = j2)
+  : Disjoint (q1 :: map fst r1) (q2 :: map fst r2).
+Proof.
+  intros x Hx1 Hx2.
+  replace (q1 :: map fst r1) with  (map fst ((q1,j1) :: r1)) in Hx1 by (cbn;eauto).
+  replace (q2 :: map fst r2) with  (map fst ((q2,j2) :: r2)) in Hx2 by (cbn;eauto).
+  decide (deq_loop q1 x).
+  - assert (eq_loop q1 x) as Heq.
+    { cbn in Hx1. split;eauto. eapply teq_r1_incl_head_q;eauto. }
+    replace (q1 :: map fst r1) with  (map fst ((q1,j1) :: r1)) in Hx1 by (cbn;eauto).
+    replace (q2 :: map fst r2) with  (map fst ((q2,j2) :: r2)) in Hx2 by (cbn;eauto).
+    eapply in_fst in Hx1. destructH.
+    eapply in_fst in Hx2. destructH.
+    enough (b = b0).
+    { subst. eapply Tdisj;eauto. }
+    assert (| b | = depth x) as Hxb1.
+    {
+      eapply path_to_elem in Hx1;eauto. 2: eapply Tpath1. destructH.
+      eapply tag_depth_unroot in Hx0;eauto. admit.
+    }
+    assert (| b0 | = depth x) as Hxb2.
+    {
+      eapply path_to_elem in Hx2;eauto. 2: eapply Tpath2. destructH.
+      eapply tag_depth_unroot in Hx0;eauto. admit.
+    }
+    assert (b = j1) as Hbj1.
+    {
+      cbn in Hx1. destruct Hx1.
+      - inv H. reflexivity.
+      - erewrite <-take_r_geq with (n:=depth q1) at 1.
+        2: rewrite Heq,Hxb1;eauto.
+        eapply teq_tag_eq1;eauto.
+        eapply in_map with (f:=snd) in H. cbn in H. eassumption.
+    }
+    assert (b0 = j1) as Hbj2.
+    {
+      cbn in Hx2. destruct Hx2.
+      - inv H. reflexivity.
+      - erewrite <-take_r_geq with (n:=depth q1) at 1.
+        2: rewrite Heq,Hxb2;eauto.
+        rewrite Tloop. subst j2.
+        eapply TeqPaths_sym in T.
+        eapply teq_tag_eq1;eauto.
+        eapply in_map with (f:=snd) in H. cbn in H. eassumption.
+    }
+    subst. reflexivity.
+  - eapply ex_ocnc_loop in n. destructH.
+    eapply ocnc_depth in n as Hdep.
+    specialize Tpath1 as Hpath1.
+    specialize Tpath2 as Hpath2.
+    subst j2. eapply TeqPaths_sym in T as Tsym.
+    eapply in_fst in Hx1 as Hin1. destructH.
+    eapply in_fst in Hx2 as Hin2. destructH.
+    eapply path_to_elem in Hin1;eauto. destructH.
+    eapply path_to_elem in Hin2;eauto. destructH.
+    assert ((h, 0 :: j1) ∈ ϕ) as Hinϕ.
+    {
+      clear Tsym.
+      decide (h = u1).
+      - subst u1. eapply path_contains_back in Hin0.
+        specialize Tlj_eq1 as [Heq|Hentry];[exfalso|];subst.
+        + eapply tag_depth_unroot2 in Hpath1;eauto with teq.
+          destruct T. rewrite <-Tj_len in Hdep. lia.
+        + eassumption.
+      - eapply ex_entry with (p:=u1).
+        + destruct n. destruct c. exact l.
+        + eapply tag_depth_unroot2 in Hpath1 as Hdepu;eauto with teq.
+          specialize Tlj_eq1 as [Heq|Hentry].
+          * subst l1. intro N. rewrite Tj_len in Hdepu. rewrite Hdepu in Hdep.
+            eapply loop_contains_deq_loop in N. eapply deq_loop_depth in N. lia.
+          * contradict n0. destruct n. eapply eq_loop_same.
+            -- split. 2: eapply loop_contains_deq_loop;eassumption.
+               eapply deq_loop_depth_eq. 1: eapply loop_contains_deq_loop;eassumption.
+               rewrite Hentry in Hdepu. cbn in Hdepu. erewrite Tj_len in Hdepu. lia.
+            -- eapply loop_contains_loop_head;eauto.
+            -- destruct H. eapply loop_contains_loop_head;eauto. admit.
+        + eapply Hin0.
+        + eapply tag_depth_unroot2 in Hpath1;eauto with teq.
+        + setoid_rewrite <-teq_tag_eq1 at 3. 2:eapply T.
+          eapply take_take_r. admit. admit.
+        + rewrite Hdep. cbn. rewrite Tj_len. lia.
+    }
+    assert ((h, 0 :: j1) ∈ ϕ0) as Hinϕ0.
+    {
+      admit.
+    }
+    eapply Tdisj. 1,2: eapply prefix_incl;eauto.
+Admitted.
