uniana/tcfg/TcfgDom.v
@@ -1,0 +1,207 @@
+Require Export TcfgqMonotone.
+Require Import Lia.
+
+Definition sub_tag i j := |i| = |j| /\ hd 0 i <= hd 0 j /\ tl i = tl j.
+
+Lemma loop_tag_dom_eq `(C : redCFG) (h p : Lab) (i j : Tag) t
+      (Hloop : loop_contains h p)
+      (Hpath : TPath (root,start_tag) (p,i) t)
+      (Htagle : j = take_r (depth h) i)
+      (Hdep : |j| = depth h)
+  : (h,j) ∈ t.
+Proof.
+  subst j.
+  clear Hdep.
+  revert h p i Hloop Hpath.
+  induction t;intros.
+  + inv Hpath.
+  + unfold TPath in Hpath. path_simpl' Hpath. destruct t.
+    {
+      eapply path_single in Hpath. destruct Hpath.
+      inversion H. subst p i. eapply root_no_loop in Hloop. contradiction.
+    }
+    inv_path Hpath. destruct c as [q j].
+    specialize (IHt) with (p:=q) (i:=j).
+    eapply tcfg_edge_destruct' in H0.
+    destruct H0 as [H0|[H0|[H0|H0]]].
+    all: destruct H0 as [Htag Hedge].
+    * subst. right.
+      eapply IHt. all:cycle 1.
+      -- eapply H.
+      -- eapply basic_edge_eq_loop in Hedge. rewrite Hedge. assumption.
+    * eapply deq_loop_entry_or in Hedge;eauto.
+      destruct Hedge.
+      -- subst. right.
+         rewrite take_r_cons_drop.
+         2: {
+           eapply loop_contains_deq_loop in H0.
+           eapply tag_depth' in H. rewrite H.
+           eapply deq_loop_depth;eauto.
+         }
+         eapply IHt;eauto.
+      -- subst p. left. rewrite take_r_geq;eauto.
+         eapply tag_depth' in Hpath. lia.
+    * destruct j.
+      {
+        eapply tag_depth' in H. cbn in H. eapply loop_contains_depth_lt in Hloop.
+        eapply back_edge_eq_loop in Hedge. rewrite Hedge in H. lia.
+      }
+      cbn in Htag. subst i.
+      decide (h = p).
+      -- subst p. left. rewrite take_r_geq;eauto.
+         eapply tag_depth' in Hpath. lia.
+      -- right. rewrite take_r_cons_replace with (b:=n).
+         2: {
+           copy Hedge Hedge'.
+           eapply back_edge_eq_loop in Hedge.
+           copy Hloop Hloop'.
+           eapply loop_contains_deq_loop in Hloop.
+           eapply eq_loop1 in Hloop;eauto. 2: symmetry;eauto.
+           eapply tag_depth' in H.
+           enough (depth h < S (| j |)).
+           { cbn in H. rewrite H in H0. lia. }
+           eapply deq_loop_depth in Hloop.
+           eapply le_lt_or_eq in Hloop.
+           destruct Hloop.
+           ++ cbn in H. lia.
+           ++ exfalso. rewrite Hedge in H0.
+              eapply loop_contains_deq_loop in Hloop' as Hdeq.
+              eapply deq_loop_depth_eq in H0;eauto.
+              eapply n0. eapply head_unique;eauto.
+              ** eapply loop_contains_ledge;eauto.
+              ** split;eauto.
+         }
+         eapply IHt;eauto.
+         eapply back_edge_eq_loop in Hedge. rewrite Hedge. eauto.
+    * subst.
+      destruct j.
+      {
+        eapply tag_depth' in H. cbn in H. eapply loop_contains_depth_lt in Hloop.
+        destruct Hedge. eapply deq_loop_exited in H0. eapply deq_loop_depth in H0. lia.
+      }
+      right. rewrite <-take_r_cons_drop with (a:=n).
+      all: cbn.
+      2: {
+        eapply tag_depth' in H. cbn in H.
+        enough (depth h < S (|j|)) by lia.
+        rewrite H.
+        eapply depth_exit in Hedge.
+        eapply loop_contains_deq_loop in Hloop. eapply deq_loop_depth in Hloop.
+        lia.
+      }
+      eapply IHt;eauto.
+      destruct Hedge. eapply deq_loop_exited in H0. eapply H0. eauto.
+Qed.
+
+Lemma loop_tag_dom_same `(C : redCFG) (h : Lab) (i j : Tag) t
+      (Hloop : loop_head h)
+      (Hpath : TPath (root,start_tag) (h,i) t)
+      (Htagle : sub_tag j i)
+  : (h,j) ∈ t.
+Proof.
+  destruct Htagle as [Hlen [Hhd Htl]].
+  destruct i,j;cbn in *;[|congruence|congruence|].
+  { eapply tag_depth' in Hpath. cbn in Hpath. eapply depth_loop_head in Hloop. lia. }
+  subst j. clear Hlen.
+  revert t Hpath.
+  induction Hhd;intros.
+  - eapply path_contains_front;eauto.
+  - destruct t;[inv Hpath|].
+    unfold TPath in Hpath. path_simpl' Hpath.
+    inversion Hpath. subst.
+    destruct b as [q j].
+    eapply tcfg_edge_destruct' in H3.
+    destruct H3 as [H3|[H3|[H3|H3]]].
+    all: destruct H3 as [Htag Hedge].
+    * eapply basic_edge_no_loop2 in Hedge. contradiction.
+    * inv Htag.
+    * destruct j;cbn in Htag;[congruence|].
+      inv Htag.
+      right.
+      eapply loop_tag_dom_eq in H0 as Hel2;cycle 1.
+      -- eapply loop_contains_ledge;eassumption.
+      -- rewrite take_r_geq;eauto. eapply tag_depth' in H0. rewrite H0.
+         eapply back_edge_eq_loop in Hedge. rewrite Hedge. eauto.
+      -- eapply back_edge_eq_loop in Hedge. rewrite <-Hedge. eapply tag_depth' in H0. eauto.
+      -- eapply path_to_elem in Hel2;eauto. destructH.
+         eapply prefix_incl;[eauto|].
+         eapply IHHhd;eassumption.
+    * destruct j;cbn in Htag;[congruence|]. subst j. destruct Hedge.
+      eapply no_exit_head in H. contradiction.
+Qed.
+
+(* could be generalized with sub_tag _ _  -> sub_tag _ _ \/ Prefix _ _ *)
+Lemma loop_tag_dom `(C : redCFG) (h p : Lab) (i j : Tag) t
+      (Hloop : loop_contains h p)
+      (Hpath : TPath (root,start_tag) (p,i) t)
+      (Hstag : sub_tag j (take_r (depth h) i))
+      (Hdep : |j| = depth h)
+  : (h,j) ∈ t.
+Proof.
+  assert (depth h <= | i |) as Hdepi.
+  {
+    eapply tag_depth' in Hpath. rewrite Hpath.
+    eapply deq_loop_depth.
+    eapply loop_contains_deq_loop;eauto.
+  }
+  eapply loop_tag_dom_eq in Hpath as Hel2.
+  3: reflexivity.
+  2: eauto.
+  2: rewrite take_r_length_le;eauto.
+  eapply path_to_elem in Hel2;eauto.
+  destructH.
+  eapply prefix_incl;eauto.
+  eapply loop_tag_dom_same;eauto.
+  eapply loop_contains_loop_head;eauto.
+Qed.
+
+Lemma tpath_deq_no_haed_tag_eq `(C : redCFG) p q q0 i j t
+      (Hlen : | j | = depth q)
+      (Hpath : TPath (q,j) (p,i) t)
+      (Hincl : forall x, x ∈ map fst t -> deq_loop x q0)
+      (Hnback : forall x : Lab, x ∈ (map fst t) -> ~ loop_contains x q0)
+  : take_r (depth q0) i = take_r (depth q0) j.
+Proof.
+  revert q p i j Hpath Hlen.
+  induction t;intros;inv_path Hpath.
+  - reflexivity.
+  - exploit' IHt.
+    { intros. eapply Hincl. cbn. right;eauto. }
+    exploit' IHt.
+    { intros. eapply Hnback. cbn. right. eauto. }
+    destruct x as [e l].
+    eapply tcfg_edge_destruct' in H0.
+    destruct H0 as [H0|[H0|[H0|H0]]].
+    all: destruct H0 as [Htag Hedge];subst.
+    + eapply IHt;eauto.
+    + rewrite take_r_cons_drop.
+      * eapply IHt;eauto.
+      * eapply tag_depth_unroot in H as Hdep;eauto. rewrite Hdep.
+        eapply deq_loop_depth. eapply Hincl. cbn. right.
+        eapply path_contains_front in H. eapply in_map with (f:=fst) in H. eauto.
+    + destruct l;[exfalso|].
+      * eapply loop_contains_ledge in Hedge. eapply loop_contains_depth_lt in Hedge.
+        eapply tag_depth_unroot in H;eauto. cbn in H. lia.
+      * cbn in Hpath. cbn.
+        erewrite take_r_cons_replace.
+        -- eapply IHt;eauto.
+        -- specialize (Hnback p). exploit Hnback. 1: cbn;left;auto.
+           decide (S (|l|) <= depth q0);[exfalso|lia].
+           eapply tag_depth_unroot in H as Hdep;eauto. cbn in Hdep. rewrite Hdep in l0.
+           assert (deq_loop e q0) as Hdeq.
+           {
+             eapply Hincl. cbn. right. eapply path_contains_front in H.
+             eapply in_map with (f:=fst) in H. cbn in H. assumption.
+           }
+           eapply deq_loop_depth_leq in l0;eauto.
+           eapply Hnback. eapply deq_loop_head_loop_contains;eauto.
+           ++ eapply back_edge_eq_loop in Hedge. rewrite <-Hedge. eauto.
+           ++ eexists;eauto.
+    + destruct l;[exfalso|].
+      * eapply tag_depth_unroot in H;eauto. cbn in H. eapply depth_exit in Hedge. lia.
+      * cbn. cbn in Hpath.
+        erewrite <-take_r_cons_drop.
+        -- eapply IHt;eauto.
+        -- eapply tag_depth_unroot in Hpath;eauto. rewrite Hpath.
+           eapply deq_loop_depth. eapply Hincl;cbn. eauto.
+Qed.
